@prefix rdf: <http://www.w3.org/1999/02/22-rdf-syntax-ns#> .
@prefix rdfs: <http://www.w3.org/2000/01/rdf-schema#> .
@prefix sage: <http://sage.univ-nantes.fr/sage-voc#> .
@prefix sd: <http://www.w3.org/ns/sparql-service-description#> .
@prefix void: <http://rdfs.org/ns/void#> .

sage:SageEndpoint a rdf:Class ;
  rdfs:subClassOf sd:Service ;
  rdfs:label "Sage endpoint"@en ;
  rdfs:comment "A Sage endpoint, which hosts several RDF datasets"@en ;
  rdfs:comment "Un point d'accès Sage, qui héberge plusieurs Datasets RDF"@fr .

sage:SageDataset a rdf:Class ;
  rdfs:subClassOf sd:Graph ;
  rdfs:subClassOf void:Dataset ;
  rdfs:label "Sage RDF dataset"@en ;
  rdfs:comment "A RDF dataset that can be queried through a Sage interface"@en ;
  rdfs:comment "Un Dataset RDF qui peux être interrogé via une interface Sage"@fr .

sage:ExampleQuery a rdf:Class ;
  rdfs:label "Example SPARQL query"@en ;
  rdfs:comment "A SPARQL query that can be run using a RDF Dataset hostyed by a Sage endpoint"@en ;
  rdfs:comment "Une requête SPARQL, qui peut être évaluée avec un Dataset RDF hébergé par un point d'accès Sage"@fr .

sage:exampleQuery a rdf:Property ;
  rdfs:domain sage:SageDataset ;
  rdfs:range sage:ExampleQuery ;
  rdfs:label "has an example query"@en ;
  rdfs:comment "Link a Sage Dataset to an example query"@en ;
  rdfs:comment "Relie un Dataset à une requête d'exemple"@fr .

sage:quota a rdf:Property ;
  rdfs:domain sage:SageDataset ;
  rdfs:range rdfs:Literal ;
  rdfs:label "use the time quota"@en ;
  rdfs:comment "Indicates the time quota used by a Sage Dataset (in milliseconds)"@en ;
  rdfs:comment "Indique le quota en time utilisé par un Dataset Sage (en millisecondes)"@fr .
